Ajustes em provas e definições.

Equation_C.v
@@ -1,8 +1,7 @@
 Require Import Arith Metatheory.
-Require Import LibTactics LambdaES_Tac.
-Require Import LambdaES_Defs LambdaES_FV LambdaES_Infra.
-Require Import Rewriting_Defs Rewriting_Lib.
-Require Import Morphisms.
+Require Import LibTactics LambdaES_Defs Rewriting.
+Require Import LambdaES_FV LambdaES_Infra LambdaES_Tac.
+Require Export Morphisms.
 
 Instance iff_eq : Equivalence iff.
 Proof. 
@@ -15,38 +14,35 @@ Qed.
 
 (** =e definition: The equation c defines permutation of independent substitutions, which corresponds to forbid dangling deBruijn indexes in both u and v, i.e. u and v are terms.  *)
 Inductive eqc : pterm -> pterm -> Prop := 
-  | eqc_rf: forall u, eqc u u  
-  | eqc_rx: forall t u v, 
-    term u -> term v -> eqc (t[u][v]) ((& t)[v][u]) 
- .
-
+  | eqc_def: forall t u v, term u -> term v -> eqc (t[u][v]) ((& t)[v][u]).
+  
 Lemma eqc_sym : forall t u, eqc t u -> eqc u t.
 Proof.
- intros t u H. destruct H. 
- apply eqc_rf. replace (t[u][v]) with ((& (& t))[u][v]).
- apply eqc_rx; trivial.
- unfold bswap. rewrite bswap_rec_id. trivial.
+ intros t u H. inversion H; subst. 
+ replace t0 with (&(& t0)) at 2.
+ apply eqc_def; assumption. 
+ apply bswap_idemp.
 Qed.
 
+(*
 Lemma eqc_trans: forall t u v, eqc t u -> eqc u v -> eqc t v.
 Proof.
  intros t u v H1 H2.
- destruct H1. trivial. inversion H2.
- apply eqc_rx; trivial. unfold bswap.
- rewrite bswap_rec_id. apply eqc_rf. 
+ destruct H1. inversion H2; subst.
+ rewrite bswap_idemp.
+ apply eqc_rf. 
 Qed.
 
-Instance eqc_eq : Equivalence eqc.
+Instance eqc_equiv : Equivalence eqc.
 Proof.
  split; intros_all.
  apply eqc_rf.
  apply eqc_sym; trivial.
  generalize H H0. apply eqc_trans.
 Qed.
+ *)
 
-(***)
-
-Definition eqC (t : pterm) (u : pterm) := trans_closure (p_contextual_closure eqc) t u.
+Definition eqC (t : pterm) (u : pterm) := star_closure (ES_contextual_closure eqc) t u.
 Notation "t =e u" := (eqC t u) (at level 66). 
 
 (** =e is an equivalence relation *)
@@ -54,31 +50,41 @@ Notation "t =e u" := (eqC t u) (at level 66).
 Lemma eqC_rf : forall t, t =e t.
 Proof.
  intro t. 
- apply one_step_reduction.
- apply p_redex. reflexivity.
+ apply reflexive_reduction.
 Qed.
 
-Lemma pctx_eqc_sym : forall t u, (p_contextual_closure eqc t u) -> p_contextual_closure eqc u t. 
+Lemma ESctx_eqc_sym : forall t u, (ES_contextual_closure eqc t u) -> ES_contextual_closure eqc u t. 
 Proof.
   intros t u H. induction H.
-  apply p_redex. rewrite H. reflexivity.
-  apply p_app; trivial.
-  apply p_abs_in with (L:=L); trivial.
-  apply p_subst with (L:=L); trivial.
+  apply ES_redex.
+  apply eqc_sym; assumption.
+  apply ES_app_left; trivial.
+  apply ES_app_right; trivial.
+  apply ES_abs_in with (L:=L); trivial.
+  apply ES_subst_left with (L:=L); trivial.
+  apply ES_subst_right; trivial.
 Qed.
 
 Lemma eqC_sym : forall t u, t =e u -> u =e t.
 Proof.
  intros t u H. induction H.
- apply one_step_reduction. apply pctx_eqc_sym; trivial.
- apply transitive_closure_composition with (u := u); trivial.
- apply one_step_reduction. apply pctx_eqc_sym; trivial.
+ apply reflexive_reduction.
+ induction H.
+ apply ESctx_eqc_sym in H.
+ apply star_trans_reduction.
+ apply one_step_reduction; assumption.
+ apply ESctx_eqc_sym in H.
+ apply star_trans_reduction.
+ inversion IHtrans_closure; subst.
+ apply one_step_reduction; assumption.
+ apply transitive_closure_composition with u. assumption.
+ apply one_step_reduction; assumption.
 Qed.
 
 Lemma eqC_trans : forall t u v, t =e u -> u =e v -> t =e v.
 Proof.
  intros t u v H H'.
- apply transitive_closure_composition with (u := u); trivial.
+ apply star_closure_composition with u; trivial.
 Qed.
 
 Instance eqC_eq : Equivalence eqC.
@@ -86,10 +92,16 @@ Proof.
  split; intros_all.
  apply eqC_rf.
  apply eqC_sym; trivial.
- apply eqC_trans with (u := y); trivial.
+ apply eqC_trans with y; trivial.
 Qed.
 
-(*** =e inversion ***)
+(*** =e inversion *)
+
+(*
+Lemma eqc_bvar_term  : forall x t, eqc (pterm_bvar x) t -> pterm_bvar x = t.
+Proof.
+  intros x t H. inversion H. trivial.
+Qed.
 
 Lemma eqc_fvar_term  : forall x t, eqc (pterm_fvar x) t -> pterm_fvar x = t.
 Proof.
@@ -107,7 +119,6 @@ Proof.
    intros t t' H. inversion H. trivial.
 Qed.
 
-
 Lemma eqc_sub_term :  forall t u t0, eqc (t[u]) t0 -> 
 (t[u] = t0 \/ exists t', exists v, term u /\ term v /\ t'[v] = t /\ (& t')[u][v] = t0) .
 Proof. 
@@ -116,65 +127,104 @@ Proof.
    split; trivial. split; trivial. split; trivial.
 Qed.
 
-(****)
-
-Lemma pctx_eqc_fvar_term  : forall x t, p_contextual_closure eqc (pterm_fvar x) t -> pterm_fvar x = t.
+Lemma ESctx_eqc_bvar_term  : forall x t, ES_contextual_closure eqc (pterm_bvar x) t -> pterm_bvar x = t.
 Proof.
   intros x t H. inversion H. inversion H0; trivial.
 Qed.
 
-Lemma pctx_eqc_app_term :  forall t u v, p_contextual_closure eqc (pterm_app u v) t ->
-                           exists u', exists v', pterm_app u' v' = t /\ p_contextual_closure eqc u' u /\ p_contextual_closure eqc v' v.
-Proof. 
-   intros t u v H. inversion H.
-   exists u v. split; trivial. inversion H0; trivial.
-   split; apply p_redex; reflexivity.
-   exists t' u'. split; trivial. 
-   split; apply pctx_eqc_sym; trivial.
+Lemma ESctx_eqc_fvar_term  : forall x t, ES_contextual_closure eqc (pterm_fvar x) t -> pterm_fvar x = t.
+Proof.
+  intros x t H. inversion H. inversion H0; trivial.
 Qed.
 
-Lemma pctx_eqc_abs_term :  forall t t', p_contextual_closure eqc (pterm_abs t) t' ->
-                       exists u, exists L, pterm_abs u = t' /\ (forall x, x \notin L -> p_contextual_closure eqc (u ^ x) (t ^ x)).
+Lemma ESctx_eqc_app_term :  forall t u v, ES_contextual_closure eqc (pterm_app u v) t -> ((exists v', t = pterm_app u v' /\ ES_contextual_closure eqc v v') \/ (exists u', t = pterm_app u' v /\ ES_contextual_closure eqc u u')).
 Proof. 
-   intros t t' H. inversion H. 
-   exists t {}. split; trivial. inversion H0; trivial.
-   intros x H'. apply p_redex. reflexivity.
+  intros t u v H. inversion H; subst.
+  apply eqc_app_term in H0. subst.
+  left. exists v.
+  split; trivial.
+  apply ES_redex. reflexivity.
+  right. exists t'. split. reflexivity. assumption.
+  left. exists u'.
+  split. reflexivity. assumption.
+Qed.
+
+Lemma ESctx_eqc_abs_term :  forall t t', ES_contextual_closure eqc (pterm_abs t) t' ->
+                       exists u, exists L, pterm_abs u = t' /\ (forall x, x \notin L -> ES_contextual_closure eqc (u ^ x) (t ^ x)).
+Proof. 
+   intros t t' H. inversion H; subst. 
+   exists t {}. split; trivial.
+   apply eqc_abs_term in H0; assumption.
+   intros x H'. apply ES_redex. reflexivity.
    exists t'0 L. split; trivial. intros. 
-   apply pctx_eqc_sym. apply H1. trivial.
+   apply ESctx_eqc_sym. apply H1; assumption.
 Qed.
 
-(**)
-
-Lemma pctx_eqc_sub_term :  forall t u t0, p_contextual_closure eqc (t[u]) t0 -> exists t', exists u', t'[u'] = t0 .
+Lemma ESctx_eqc_sub_term :  forall t u v, ES_contextual_closure eqc (t[u]) v -> exists t', exists u', v = (t'[u']).
 Proof. 
-   intros t u t0 H. inversion H. inversion H0.
-   exists t u; trivial. 
-   exists (& t2 [u]) u0; trivial.
-   exists t' u'; trivial.
+  intros t u v H. inversion H; subst.
+  apply eqc_sub_term in H0.
+  destruct H0. subst.
+  exists t u; trivial. 
+  destruct H0. destruct H0. destruct H0. destruct H1. destruct H2. subst.
+  exists (& x [u]) x0; trivial.
+  exists t' u; trivial.
+  exists t u'; reflexivity.
 Qed.
 
-(**)
-
-(****)
+Lemma eqC_bvar_term  : forall x t, pterm_bvar x =e t -> pterm_bvar x = t.
+Proof.
+  intros x t H. gen_eq t0 : (pterm_bvar x). induction H.
+  intro H'. subst.  
+  apply ESctx_eqc_bvar_term in H; assumption.
+  intro H'. subst.
+  rewrite <- IHtrans_closure.
+  apply ESctx_eqc_bvar_term in H; assumption.
+  symmetry.
+  apply ESctx_eqc_bvar_term in H; assumption.
+Qed.
 
 Lemma eqC_fvar_term  : forall x t, pterm_fvar x =e t -> pterm_fvar x = t.
 Proof.
   intros x t H. gen_eq t0 : (pterm_fvar x). induction H.
-  intro H'. rewrite H' in *|-*. apply pctx_eqc_fvar_term; trivial.
-  intro H'. rewrite H' in *|-*. rewrite <- IHtrans_closure.
-  apply pctx_eqc_fvar_term; trivial. 
-  apply pctx_eqc_fvar_term in H. rewrite H; trivial.
+  intro H'. subst.
+  apply ESctx_eqc_fvar_term; trivial.
+  intro H'. subst.
+  rewrite <- IHtrans_closure.
+  apply ESctx_eqc_fvar_term; trivial. 
+  apply ESctx_eqc_fvar_term in H. rewrite H; trivial.
 Qed.
 
 Lemma eqC_app_term :  forall t u v, pterm_app u v =e t ->
-                      exists u', exists v', pterm_app u' v' = t /\ u' =e u /\ v' =e v.
-Proof. 
-  intros t u v H. gen_eq t0 : (pterm_app u v). generalize u v. clear u v. induction H.
-  intros u0 v0 H'. rewrite H' in *|-*. apply pctx_eqc_app_term in H.
-  case H; clear H; intros u' H. case H; clear H; intros v' H. destruct H. destruct H0.
-  exists u' v'. split; trivial. split; apply one_step_reduction; trivial.
-  intros u0 v0 H'. rewrite H' in H. apply pctx_eqc_app_term in H.
-  case H; clear H; intros u1 H. case H; clear H; intros v1 H. destruct H. destruct H1.
+                      exists u', exists v', t = pterm_app u' v' /\ u' =e u /\ v' =e v.
+Proof.(* aqui *) 
+  intros t u v H. remember (pterm_app u v) as t'.
+  generalize dependent u.
+  generalize dependent v.
+  induction H.
+  intros v u' H'. subst.
+  exists u' v.
+  split.
+  apply ESctx_eqc_app_term in H.
+  destruct H. destruct H. destruct H. subst.
+  
+  intros u0 v0 H'. rewrite H' in *. apply ESctx_eqc_app_term in H.
+  case H; clear H. intro H. case H; clear H; intros v' H. destruct H. 
+  exists u0 v'. split; trivial.
+  split.
+  reflexivity.
+  apply one_step_reduction. apply ESctx_eqc_sym; assumption.
+  intro H.
+  destruct H. destruct H.
+  exists x v0. split. assumption.
+  split.
+  apply one_step_reduction. apply ESctx_eqc_sym; assumption. reflexivity.
+  intros u0 v0 H'. apply IHtrans_closure. subst.
+  apply ESctx_eqc_app_term in H.
+  case H; clear H.
+  intro H. destruct H. destruct H.
+  rewrite H.
+  intros u1 H. case H; clear H; intros v1 H. destruct H. destruct H1.
   case (IHtrans_closure u1 v1). rewrite H; trivial. intros u2 H3.
   case H3; clear H3; intros v2 H3. destruct H3. destruct H4.
   exists u2 v2. split; trivial. 
@@ -196,9 +246,6 @@ Proof.
    rewrite (H3 x); trivial. apply one_step_reduction. apply H1; trivial.
 Qed.
 
-
-(***)
-
 Lemma eqC_sub_term :  forall t u t0, t[u] =e t0 -> exists t', exists u', t'[u'] = t0 .
 Proof. 
    intros t u v H. gen_eq t0 : (t [u]). generalize t u; clear t u. induction H.
@@ -209,21 +256,19 @@ Proof.
    case H1; clear H1; intros u1 H1. exists t1 u1; trivial.
 Qed.
 
-
-
 Lemma eqC_redex : forall t u v, term u -> term v -> (t[u][v]) =e ((& t)[v][u]) .
 Proof.
  intros t u v Tu Tv. apply one_step_reduction. apply p_redex. apply eqc_rx; trivial.
 Qed.
-
+*)
 
 Definition red_ctx_mod_eqC (R: pterm -> pterm -> Prop) (t: pterm) (u : pterm) := 
-           exists t', exists u', (t =e t')/\(contextual_closure R t' u')/\(u' =e u).
+           exists t', exists u', (t =e t')/\(ES_contextual_closure R t' u')/\(u' =e u).
 
 
 (* ********************************************************************** *)
 (** =e Properties *)
-
+(*
 Lemma lc_at_eqc : forall n t u, eqc t u  -> (lc_at n t <-> lc_at n u).
 Proof.
  intros n t u H. destruct H; split; simpl; trivial.
@@ -585,30 +630,37 @@ Proof.
   rewrite subst_intro with (x := x); trivial.
   rewrite subst_intro with (x := x) (t := t2); trivial.
 Qed.
-
+*)
 (* ********************************************************************** *)
 (** =e Rewriting *)
 
 Instance rw_eqC_red : forall R, Proper (eqC ==> eqC ==> iff) (red_ctx_mod_eqC R).
 Proof.
  intros_all. split. intro H1.
- unfold red_ctx_mod_eqC in *|-*.
+ unfold red_ctx_mod_eqC in *.
  destruct H1. destruct H1. destruct H1. destruct H2.
- exists x1. exists x2. split. 
- rewrite <- H; trivial. split; trivial.
- rewrite <- H0; trivial. intro H1.
- unfold red_ctx_mod_eqC in *|-*.
+ exists x1 x2. split. 
+ apply eqC_sym in H.
+ apply eqC_trans with x; assumption.
+ split. assumption.
+ apply eqC_trans with x0; assumption.
+ intro H1.
+ unfold red_ctx_mod_eqC in *.
  destruct H1. destruct H1. destruct H1. destruct H2.
- exists x1. exists x2. split. 
- rewrite <- H1; trivial. split; trivial.
+ exists x1 x2. split. 
+ rewrite <- H1; assumption. split; trivial.
  rewrite H3. rewrite H0. 
  reflexivity.
 Qed.
 
 Instance rw_eqC_trs : forall R, Proper (eqC ==> eqC ==> iff) (trans_closure (red_ctx_mod_eqC R)).
-Proof.
- intros_all. split. intro H'.
- apply transitive_star_derivation'.
+Proof. (* Lucas *)
+  intros_all. split. intro H'.
+  apply transitive_reduction with x0.
+  inversion H'; subst.
+  exists x x0.
+  split. apply eqC_sym; assumption.
+  split.  apply transitive_star_derivation'.
  apply transitive_star_derivation' in H'.
  case H'. clear H'. intro H1. left.
  rewrite <- H. rewrite <- H0; trivial.
@@ -670,6 +722,7 @@ Proof.
  apply p_redex. apply eqc_rf.
 Qed.
 
+(*
 Instance SN_ind_mod_eqC : forall n R, Proper (eqC ==> iff) (SN_ind n (red_ctx_mod_eqC R)).
 Proof.
  intros_all. split. intro H'.
@@ -689,10 +742,10 @@ Proof.
  intros t0 H0. rewrite H in H0.
  apply (H' t0); trivial. 
 Qed.
-
+*)
 
 (* ********************************************************************** *)
-
+(*
 Lemma ctx_to_mod_eqC : forall R t t', contextual_closure R t t' -> red_ctx_mod_eqC R t t'.
 Proof.
  intros R t t' H. 
@@ -1132,8 +1185,7 @@ Inductive eqC'  : pterm -> pterm -> Prop :=
     eqC' (pterm_abs t) (pterm_abs t') 
   | eqC'_sub : forall t t' u u' L,   
    (forall x, x \notin L -> eqC' (t ^ x) (t' ^ x)) -> eqC' u u' ->  
-    eqC' (t[u]) (t'[u'])
-. 
+    eqC' (t[u]) (t'[u']). 
 
  Notation "t =e' u" := (eqC' t u) (at level 66). 
 
@@ -1428,5 +1480,5 @@ Proof.
   reflexivity.
 Qed.
 
-
+*)
 
